Example proofs for []byte fields

example/event.go
@@ -6,6 +6,7 @@ import (
 
 type Event struct {
 	id        uint32
+	name      *[]byte
 	startTime *TimeStamp
 	endTime   *TimeStamp
 }
@@ -17,6 +18,10 @@ func (e *Event) approxSize() uint64 {
 func MarshalEvent(e *Event, prefix []byte) []byte {
 	var enc = prefix
 	enc = marshal.WriteInt32(enc, e.id)
+
+	enc = marshal.WriteInt(enc, uint64(len(*e.name)))
+	enc = marshal.WriteBytes(enc, *e.name)
+
 	enc = MarshalTimeStamp(e.startTime, enc)
 	enc = MarshalTimeStamp(e.endTime, enc)
 	return enc
@@ -26,6 +31,13 @@ func UnmarshalEvent(s []byte) (*Event, []byte) {
 	e := new(Event)
 	var enc = s // Needed for goose compatibility
 	e.id, enc = marshal.ReadInt32(enc)
+
+	var nameLen uint64
+	var name []byte
+	nameLen, enc = marshal.ReadInt(enc)
+	name, enc = marshal.ReadBytesCopy(enc, nameLen)
+	e.name = &name
+
 	e.startTime, enc = UnmarshalTimeStamp(enc)
 	e.endTime, enc = UnmarshalTimeStamp(enc)
 	return e, enc
